Remove redundant CavaExpr in favor of Kappa (#186)
- Add evaluation semantics for @Kappa Cava combinational expressions
- Standardise CavaArrow methods to have right most unit (reduces the amount of conversion functions needed).

cava/cava/Cava/Arrow/ArrowKind.v
@@ -185,3 +185,19 @@ match ty with
 | Tuple l r => Tuple l (remove_rightmost_unit r)
 | x => x
 end.
+
+Fixpoint denote_kind (ty: Kind): Type :=
+  match ty with 
+  | Tuple l r => denote_kind l * denote_kind r
+  | Bit => bool
+  | Vector ty n => Vector.t (denote_kind ty) n
+  | Unit => unit
+  end.
+
+Fixpoint kind_default (ty: Kind): denote_kind ty :=
+  match ty return denote_kind ty with 
+  | Tuple l r => (kind_default l, kind_default r)
+  | Bit => false
+  | Vector ty n => const (kind_default ty) n
+  | Unit => tt
+  end.
